support (pure) invariants associated with GC locations

theories/heap_lang/lib/gc.v
@@ -6,11 +6,15 @@ Set Default Proof Using "Type".
 Import uPred.
 
 (** A "GC" location is a location that can never be deallocated explicitly by
-the program.  It provides a persistent witness that wuill always allow reading
-the location, albeit with no way to predict what is going to be read.  This is
-useful for data structures like RDCSS that need to read locations long after
-their ownership has been passed back to the client, but do not care *what* it is
-that they are reading in that case.
+the program.  It provides a persistent witness that will always allow reading
+the location.  The location is moreover associated with a (pure, Coq-level)
+invariant determining which values are allowed to be stored in that location.
+The persistent witness cannot know the exact value that will be read, but it
+*can* know that the value satisfies the invariant.
+
+This is useful for data structures like RDCSS that need to read locations long
+after their ownership has been passed back to the client, but do not care *what*
+it is that they are reading in that case.
 
 Note that heap_lang does not actually have explicit dealloaction. However, the
 proof rules we provide for heap operations currently are conservative in the
@@ -18,11 +22,16 @@ sense that they do not expose this fact.  By making "GC" locations a separate
 assertion, we can keep all the other proofs that do not need it conservative.
 *)
 
+Local Notation loc_inv := (val → Prop).
+
 Definition gcN: namespace := nroot .@ "gc".
 
-Definition gc_mapUR : ucmraT := gmapUR loc $ optionR $ exclR $ valO.
+Definition gc_mapUR : ucmraT := gmapUR loc $ prodR
+  (optionR $ exclR $ valO)
+  (agreeR $ leibnizO loc_inv).
 
-Definition to_gc_map (gcm: gmap loc val) : gc_mapUR := (λ v : val, Excl' v) <$> gcm.
+Definition to_gc_map (gcm: gmap loc (val * loc_inv)) : gc_mapUR :=
+  (λ p: val * loc_inv, (Excl' p.1, to_agree p.2)) <$> gcm.
 
 Class gcG  (Σ : gFunctors) := GcG {
   gc_inG :> inG Σ (authR (gc_mapUR));
@@ -45,30 +54,34 @@ Section defs.
 
   Context `{!invG Σ, !heapG Σ, gG: gcG Σ}.
 
-  Definition gc_inv_P: iProp Σ := 
-    ((∃(gcm: gmap loc val), own (gc_name gG) (● to_gc_map gcm) ∗ ([∗ map] l ↦ v ∈ gcm, (l ↦ v)) ) )%I.
+  Definition gc_inv_P : iProp Σ :=
+    (∃ gcm : gmap loc (val * loc_inv),
+        own (gc_name gG) (● to_gc_map gcm) ∗ ([∗ map] l ↦ p ∈ gcm, ⌜p.2 p.1⌝ ∗ (l ↦ p.1)) )%I.
 
   Definition gc_inv : iProp Σ := inv gcN gc_inv_P.
 
-  Definition gc_mapsto (l: loc) (v: val) : iProp Σ := own (gc_name gG) (◯ {[l := Excl' v]}).
+  Definition gc_mapsto (l : loc) (v : val) (I : loc_inv) : iProp Σ :=
+    own (gc_name gG) (◯ {[l := (Excl' v, to_agree I)]}).
 
-  Definition is_gc_loc (l: loc) : iProp Σ := own (gc_name gG) (◯ {[l := None]}).
+  Definition is_gc_loc (l : loc) (I : loc_inv) : iProp Σ :=
+    own (gc_name gG) (◯ {[l := (None, to_agree I)]}).
 
 End defs.
 
 Section to_gc_map.
 
-  Lemma to_gc_map_valid gcm: ✓ to_gc_map gcm.
+  Lemma to_gc_map_valid gcm : ✓ to_gc_map gcm.
   Proof. intros l. rewrite lookup_fmap. by case (gcm !! l). Qed.
 
-  Lemma to_gc_map_empty: to_gc_map ∅ = ∅.
+  Lemma to_gc_map_empty : to_gc_map ∅ = ∅.
   Proof. by rewrite /to_gc_map fmap_empty. Qed.
 
-  Lemma to_gc_map_singleton l v: to_gc_map {[l := v]} = {[l :=  Excl' v]}.
+  Lemma to_gc_map_singleton l v I :
+    to_gc_map {[l := (v, I)]} = {[l :=  (Excl' v, to_agree I)]}.
   Proof. by rewrite /to_gc_map fmap_insert fmap_empty. Qed.
 
-  Lemma to_gc_map_insert l v gcm:
-    to_gc_map (<[l := v]> gcm) = <[l := Excl' v]> (to_gc_map gcm).
+  Lemma to_gc_map_insert l v I gcm :
+    to_gc_map (<[l := (v, I)]> gcm) = <[l := (Excl' v, to_agree I)]> (to_gc_map gcm).
   Proof. by rewrite /to_gc_map fmap_insert. Qed.
 
   Lemma to_gc_map_delete l gcm :
@@ -79,59 +92,26 @@ Section to_gc_map.
     gcm !! l = None → to_gc_map gcm !! l = None.
   Proof. by rewrite /to_gc_map lookup_fmap=> ->. Qed.
 
-  Lemma lookup_to_gc_map_Some gcm l v :
-    gcm !! l = Some v → to_gc_map gcm !! l = Some (Excl' v).
+  Lemma lookup_to_gc_map_Some gcm l v I :
+    gcm !! l = Some (v, I) → to_gc_map gcm !! l = Some (Excl' v, to_agree I).
   Proof. by rewrite /to_gc_map lookup_fmap=> ->. Qed.
 
-
-  Lemma lookup_to_gc_map_Some_2 gcm l w :
-    to_gc_map gcm !! l = Some w → ∃ v, gcm !! l = Some v.
+  Lemma lookup_to_gc_map_Some_2 gcm l v' I' :
+    to_gc_map gcm !! l ≡ Some (v', I') → ∃ v I, v' ≡ Excl' v ∧ I' ≡ to_agree I /\ gcm !! l = Some (v, I).
   Proof.
-    rewrite /to_gc_map lookup_fmap. rewrite fmap_Some.
-    intros (x & Hsome & Heq). eauto.
-  Qed.
-
-  Lemma lookup_to_gc_map_Some_3 gcm l w :
-    to_gc_map gcm !! l = Some (Excl' w) → gcm !! l = Some w.
-  Proof.
-    rewrite /to_gc_map lookup_fmap. rewrite fmap_Some.
-    intros (x & Hsome & Heq). by inversion Heq.
-  Qed.
-
-  Lemma excl_option_included (v: val) y:
-    ✓ y → Excl' v ≼ y → y = Excl' v.
-  Proof.
-    intros ? H. destruct y.
-    - apply Some_included_exclusive in H;[ | apply _ | done ].
-      setoid_rewrite leibniz_equiv_iff in H.
-      by rewrite H.
-    - apply is_Some_included in H.
-      + by inversion H.
-      + by eapply mk_is_Some.
-  Qed.
-
-  Lemma gc_map_singleton_included gcm l v :
-    {[l := Some (Excl v)]} ≼ to_gc_map gcm → gcm !! l = Some v.
-  Proof.
-    rewrite singleton_included.
-    setoid_rewrite Some_included_total.
-    intros (y & Hsome & Hincluded).
-    pose proof (lookup_valid_Some _ _ _ (to_gc_map_valid gcm) Hsome) as Hvalid.
-    pose proof (excl_option_included _ _ Hvalid Hincluded) as Heq.
-    rewrite Heq in Hsome.
-    apply lookup_to_gc_map_Some_3.
-    by setoid_rewrite leibniz_equiv_iff in Hsome.
+    rewrite /to_gc_map lookup_fmap. rewrite fmap_Some_equiv.
+    intros ([] & Hsome & [Heqv HeqI]). eauto.
   Qed.
 End to_gc_map.
 
 Lemma gc_init `{!invG Σ, !heapG Σ, !gcPreG Σ} E:
-  (|==> ∃ _ : gcG Σ, |={E}=> gc_inv)%I.
+  ⊢ |==> ∃ _ : gcG Σ, |={E}=> gc_inv.
 Proof.
   iMod (own_alloc (● (to_gc_map ∅))) as (γ) "H●".
   { rewrite auth_auth_valid. exact: to_gc_map_valid. }
   iModIntro.
   iExists (GcG Σ _ γ).
-  iAssert (gc_inv_P (gG := GcG Σ _ γ)) with "[H●]" as "P". 
+  iAssert (gc_inv_P (gG := GcG Σ _ γ)) with "[H●]" as "P".
   {
     iExists _. iFrame.
     by iApply big_sepM_empty.
@@ -142,115 +122,143 @@ Qed.
 
 Section gc.
   Context `{!invG Σ, !heapG Σ, !gcG Σ}.
+  Implicit Types (l : loc) (I : loc_inv).
 
-  Global Instance is_gc_loc_persistent (l: loc): Persistent (is_gc_loc l).
+  Global Instance is_gc_loc_persistent l I : Persistent (is_gc_loc l I).
   Proof. rewrite /is_gc_loc. apply _. Qed.
 
-  Global Instance is_gc_loc_timeless (l: loc): Timeless (is_gc_loc l).
+  Global Instance is_gc_loc_timeless l I : Timeless (is_gc_loc l I).
   Proof. rewrite /is_gc_loc. apply _. Qed.
 
-  Global Instance gc_mapsto_timeless (l: loc) (v: val): Timeless (gc_mapsto l v).
+  Global Instance gc_mapsto_timeless l v I : Timeless (gc_mapsto l v I).
   Proof. rewrite /is_gc_loc. apply _. Qed.
 
-  Global Instance gc_inv_P_timeless: Timeless gc_inv_P.
-  Proof. rewrite /gc_inv_P. apply _. Qed.
-
-  Lemma make_gc l v E: ↑gcN ⊆ E → gc_inv -∗ l ↦ v ={E}=∗ gc_mapsto l v.
+  Lemma make_gc l v I E :
+    ↑gcN ⊆ E →
+    I v →
+    gc_inv -∗ l ↦ v ={E}=∗ gc_mapsto l v I.
   Proof.
-    iIntros (HN) "#Hinv Hl".
-    iMod (inv_open_timeless _ gcN _ with "Hinv") as "[P Hclose]"=>//.
+    iIntros (HN HI) "#Hinv Hl".
+    iMod (inv_acc_timeless _ gcN _ with "Hinv") as "[P Hclose]"=>//.
     iDestruct "P" as (gcm) "[H● HsepM]".
     destruct (gcm !! l) as [v' | ] eqn: Hlookup.
     - (* auth map contains l --> contradiction *)
-      iDestruct (big_sepM_lookup with "HsepM") as "Hl'"=>//.
+      iDestruct (big_sepM_lookup with "HsepM") as "[_ Hl']"=>//.
       by iDestruct (mapsto_valid_2 with "Hl Hl'") as %?.
     - iMod (own_update with "H●") as "[H● H◯]".
       {
         apply lookup_to_gc_map_None in Hlookup.
-        apply (auth_update_alloc _ (to_gc_map (<[l := v]> gcm)) (to_gc_map ({[l := v]}))).
+        apply (auth_update_alloc _ (to_gc_map (<[l := (v, I)]> gcm)) (to_gc_map ({[l := (v, I)]}))).
         rewrite to_gc_map_insert to_gc_map_singleton.
         pose proof (to_gc_map_valid gcm).
         setoid_rewrite alloc_singleton_local_update=>//.
       }
-      iMod ("Hclose" with "[H● HsepM Hl]"). 
+      iMod ("Hclose" with "[H● HsepM Hl]").
       + iExists _.
-        iDestruct (big_sepM_insert with "[HsepM Hl]") as "HsepM"=>//; iFrame. iFrame.
+        iDestruct (big_sepM_insert with "[HsepM Hl]") as "HsepM"=>//; iFrame.
+        auto with iFrame.
       + iModIntro. by rewrite /gc_mapsto to_gc_map_singleton.
   Qed.
 
-  Lemma gc_is_gc l v: gc_mapsto l v -∗ is_gc_loc l.
+  Lemma gc_is_gc l v I : gc_mapsto l v I -∗ is_gc_loc l I.
   Proof.
     iIntros "Hgc_l". rewrite /gc_mapsto.
-    assert (Excl' v = (Excl' v) ⋅ None)%I as ->. { done. }
-    rewrite -op_singleton auth_frag_op own_op.
+    (* We need to help Coq type inference... *)
+    change loc_inv with (ofe_car $ leibnizO loc_inv) in I.
+    (* FIXME: is there any good way to avoid repeating the goal here? *)
+    assert (◯ {[l := (Excl' v, to_agree I)]} ≡ ◯ {[l := (Excl' v, to_agree I)]} ⋅ ◯ {[l := (None, to_agree I)]}) as ->.
+    { rewrite -auth_frag_op op_singleton -pair_op agree_idemp //. }
     iDestruct "Hgc_l" as "[_ H◯_none]".
     iFrame.
   Qed.
 
-  Lemma is_gc_lookup_Some  l gcm: is_gc_loc l -∗ own (gc_name _) (● to_gc_map gcm) -∗ ⌜∃ v, gcm !! l = Some v⌝.
+  Lemma is_gc_lookup_Some l gcm I :
+    is_gc_loc l I -∗ own (gc_name _) (● to_gc_map gcm) -∗ ⌜∃ v, gcm !! l = Some (v, I)⌝.
+  Proof.
     iIntros "Hgc_l H◯".
     iCombine "H◯ Hgc_l" as "Hcomb".
     iDestruct (own_valid with "Hcomb") as %Hvalid.
     iPureIntro.
-    apply auth_both_valid in Hvalid as [Hincluded Hvalid]. 
-    setoid_rewrite singleton_included in Hincluded. 
-    destruct Hincluded as (y & Hsome & _).
-    eapply lookup_to_gc_map_Some_2.
-    by apply leibniz_equiv_iff in Hsome.
+    apply auth_both_valid in Hvalid as [Hincluded Hvalid].
+    setoid_rewrite singleton_included in Hincluded.
+    destruct Hincluded as ([v' I'] & Hsome & Hincl).
+    edestruct lookup_to_gc_map_Some_2 as [v'' [I'' (_ & HI & Hgcm)]]; first done.
+    rewrite ->HI in Hincl. exists v''. rewrite Hgcm. f_equal.
+    rewrite ->Some_included_total in Hincl.
+    apply pair_included in Hincl. simpl in Hincl.
+    destruct Hincl as [_ Hincl%to_agree_included].
+    fold_leibniz. subst I''. done.
   Qed.
 
-  Lemma gc_mapsto_lookup_Some l v gcm: gc_mapsto l v -∗ own (gc_name _) (● to_gc_map gcm) -∗ ⌜ gcm !! l = Some v ⌝.
+  Lemma gc_mapsto_lookup_Some l v gcm I :
+    gc_mapsto l v I -∗ own (gc_name _) (● to_gc_map gcm) -∗ ⌜ gcm !! l = Some (v, I) ⌝.
   Proof.
     iIntros "Hgc_l H●".
     iCombine "H● Hgc_l" as "Hcomb".
     iDestruct (own_valid with "Hcomb") as %Hvalid.
     iPureIntro.
-    apply auth_both_valid in Hvalid as [Hincluded Hvalid]. 
-    by apply gc_map_singleton_included.
+    apply auth_both_valid in Hvalid as [Hincluded Hvalid].
+    setoid_rewrite singleton_included in Hincluded.
+    destruct Hincluded as ([v' I'] & Hsome & Hincl).
+    edestruct lookup_to_gc_map_Some_2 as [v'' [I'' (Hv & HI & ->)]]; first done.
+    rewrite ->HI in Hincl. f_equal.
+    rewrite ->Some_included_total in Hincl.
+    apply pair_included in Hincl. simpl in Hincl.
+    destruct Hincl as [Hinclv HinclI%to_agree_included].
+    rewrite ->Hv in Hinclv.
+    apply Excl_included in Hinclv.
+    fold_leibniz. subst. done.
   Qed.
 
   (** An accessor to make use of [gc_mapsto].
     This opens the invariant *before* consuming [gc_mapsto] so that you can use
     this before opening an atomic update that provides [gc_mapsto]!. *)
-  Lemma gc_access E:
+  Lemma gc_access E :
     ↑gcN ⊆ E →
-    gc_inv ={E, E ∖ ↑gcN}=∗ ∀ l v, gc_mapsto l v -∗
-      (l ↦ v ∗ (∀ w, l ↦ w ==∗ gc_mapsto l w ∗ |={E ∖ ↑gcN, E}=> True)).
+    gc_inv ={E, E ∖ ↑gcN}=∗ ∀ l v I, gc_mapsto l v I -∗
+      (⌜I v⌝ ∗ l ↦ v ∗ (∀ w, ⌜I w ⌝ -∗ l ↦ w ==∗ gc_mapsto l w I ∗ |={E ∖ ↑gcN, E}=> True)).
   Proof.
     iIntros (HN) "#Hinv".
-    iMod (inv_open_timeless _ gcN _ with "Hinv") as "[P Hclose]"=>//.
-    iIntros "!>" (l v) "Hgc_l".
+    iMod (inv_acc_timeless _ gcN _ with "Hinv") as "[P Hclose]"=>//.
+    iIntros "!>" (l v I) "Hgc_l".
     iDestruct "P" as (gcm) "[H● HsepM]".
     iDestruct (gc_mapsto_lookup_Some with "Hgc_l H●") as %Hsome.
-    iDestruct (big_sepM_delete with "HsepM") as "[Hl HsepM]"=>//. 
-    iFrame. iIntros (w) "Hl".
+    iDestruct (big_sepM_delete with "HsepM") as "[[HI Hl] HsepM]"=>//=.
+    iFrame. iIntros (w) "% Hl".
     iMod (own_update_2 with "H● Hgc_l") as "[H● H◯]".
-    { apply (auth_update _ _ (<[l := Excl' w]> (to_gc_map gcm)) {[l := Excl' w]}).
-      eapply singleton_local_update.
+    { apply (auth_update _ _ (<[l := (Excl' w, to_agree I)]> (to_gc_map gcm)) {[l := (Excl' w, to_agree I)]}).
+      apply: singleton_local_update.
       { by apply lookup_to_gc_map_Some in Hsome. }
-      by apply option_local_update, exclusive_local_update.
+      apply prod_local_update; simpl.
+      - by apply option_local_update, exclusive_local_update.
+      - done.
     }
-    iDestruct (big_sepM_insert with "[Hl HsepM]") as "HsepM"; [ | iFrame | ].
+    iDestruct (big_sepM_insert _ _ _ (w, I) with "[Hl HsepM]") as "HsepM"; [ | by iFrame | ].
     { apply lookup_delete. }
     rewrite insert_delete. rewrite <- to_gc_map_insert.
     iModIntro. iFrame.
     iMod ("Hclose" with "[H● HsepM]"); [ iExists _; by iFrame | by iModIntro].
-  Qed.   
+  Qed.
 
-  Lemma is_gc_access l E: ↑gcN ⊆ E → gc_inv -∗ is_gc_loc l ={E, E ∖ ↑gcN}=∗ ∃ v, l ↦ v ∗ (l ↦ v ={E ∖ ↑gcN, E}=∗ ⌜True⌝).
+  Lemma is_gc_access l I E :
+    ↑gcN ⊆ E →
+    gc_inv -∗ is_gc_loc l I ={E, E ∖ ↑gcN}=∗
+    ∃ v, ⌜I v⌝ ∗ l ↦ v ∗ (l ↦ v ={E ∖ ↑gcN, E}=∗ ⌜True⌝).
   Proof.
     iIntros (HN) "#Hinv Hgc_l".
-    iMod (inv_open_timeless _ gcN _ with "Hinv") as "[P Hclose]"=>//.
+    iMod (inv_acc_timeless _ gcN _ with "Hinv") as "[P Hclose]"=>//.
     iModIntro.
     iDestruct "P" as (gcm) "[H● HsepM]".
     iDestruct (is_gc_lookup_Some with "Hgc_l H●") as %Hsome.
     destruct Hsome as [v Hsome].
-    iDestruct (big_sepM_lookup_acc with "HsepM") as "[Hl HsepM]"=>//. 
-    iExists _. iFrame.
+    iDestruct (big_sepM_lookup_acc with "HsepM") as "[[#HI Hl] HsepM]"=>//.
+    iExists _. iFrame "∗#".
     iIntros "Hl".
     iMod ("Hclose" with "[H● HsepM Hl]"); last done.
     iExists _. iFrame.
-    by (iApply ("HsepM" with "Hl")).
+    iApply ("HsepM" with "[Hl]"). by iFrame.
   Qed.
 
 End gc.
+
+Typeclasses Opaque is_gc_loc gc_mapsto.
